src/Analysis/Domains/Sign_Side_IP_Soundness.thy
@@ -84,8 +84,8 @@ proof -
      \<le> sound_domain.gamma_state gamma_sign
          (side_analyse_ip_eff \<Pi> ps main sign_etf bot s0
            (cfg_exit (compile_prog \<Pi> ps main)))"
-    by (rule se.side_analyse_ip_eff_collect_sound_exit_pruned_gen
-          [OF sign_etf_is_mono_eq sign_etf_mono_sides sign_etf_mono_deps
+    by (rule side_analyse_ip_eff_collect_sound_exit_pruned_gen
+          [OF sign_sound_etf sign_etf_is_mono_eq sign_etf_mono_sides sign_etf_mono_deps
               side_solve_dom gs ed cd1 cd2 es cs])
   have "t \<in> sound_domain.gamma_state gamma_sign
        (side_analyse_ip_eff \<Pi> ps main sign_etf bot s0
