src/Analysis/Solver/TD_Side_IP_Eff_Bounds.thy
@@ -577,7 +577,7 @@ proof -
         = traverse_rhs (apply_etf etf a u) \<sigma> \<squnion> sides_of_rhs (apply_etf etf a u) \<sigma> (Inr ())"
     by (simp add: etf_full_def all_sides_eq_sides_Inr_unit)
   also have "\<dots> \<le> \<sigma> (Inl v) \<squnion> \<sigma> (Inr ())" using loc glob by (rule sup_mono)
-  finally show ?thesis unfolding side_env_def .
+  finally show ?thesis unfolding side_env_def glob_env_unit .
 qed
 
 lemma etf_combine_combined_le_ip_eff:
@@ -603,7 +603,7 @@ proof -
         = traverse_rhs (etf_combine etf cc ex) \<sigma> \<squnion> sides_of_rhs (etf_combine etf cc ex) \<sigma> (Inr ())"
     by (simp add: etf_full_def all_sides_eq_sides_Inr_unit)
   also have "\<dots> \<le> \<sigma> (Inl v) \<squnion> \<sigma> (Inr ())" using loc glob by (rule sup_mono)
-  finally show ?thesis unfolding side_env_def .
+  finally show ?thesis unfolding side_env_def glob_env_unit .
 qed
 
 end
